%%% EXERCISE 1.22
\HRule
\subsection*{Exercise 1.2 (The Twisted Cubic Curve)}
\subsection*{%
  Let $X=\{(t,t^2,t^3)\in\AAA^3\mid t\in k\}$. Prove that
  \begin{enumerate}
  \item  $X=\VV(y-x^2,z-x^3)$ has dimension 1.
  \item $\II(X)=\gen{y-x^2,z-x^3}$.
    \item $A(X)\cong k[x]$.
  \end{enumerate}
} 

%%% ANSWER
\begin{proof}$\;$\\
  \begin{enumerate}
  \item The inclusion $X\subseteq\VV(y-x^2,z-x^3)$ is clear. The other inclusion
    follows from
    \[
      (x,y,z)\in\VV(y-x^2,z-x^3)\quad\then\quad
      y=x^2\;\; , \;\; z=x^3 \quad\then\quad
      (x,y,z)=(x,x^2,x^3)\quad (x\in k).
    \]
  \item The inclusion $\supseteq$ is clear since $y-x^2,z-x^3\in\II(X)$. For the other
    inclusion observe that any monomial $x^{\alpha}y^{\beta}z^{\gamma}\in k[x,y,z]$ can be
    writen as
    \begin{align*}
      x^{\alpha}y^{\beta}z^{\gamma} & = x^{\alpha}(x^2+y-x^2)^{\beta}(x^3+z-x^3)^{\gamma} \\
      & = x^{\alpha}\Big( x^{2\beta}+(y-x^2)\underset{h(x,y)}%
      {\underbrace{\sum_{i=0}^{\beta-1}\binom{\beta}{i}x^{2i}(y-x^2)^{\beta-i-1}}}
    \Big) \Big(x^{3\gamma}+(z-x^3)\underset{h'(x,y)}%
    {\underbrace{\sum_{i=0}^{\gamma-1}\binom{\gamma}{i}x^{3i}(z-x^3)^{\gamma-i-1}}}\Big)\\
    & = x^{\alpha+2\beta+3\gamma}+(y-x^2)\big(\underset{h_1(x,y,z)}%
    {\underbrace{x^{\alpha+3\gamma}h(x,y)+(z-x^3)x^{\alpha}h(x,y)h'(x,y)}} \big)+
    (z-x^3)\big(\underset{h_2(x,y,z)}{\underbrace{x^{\alpha+2\beta}h'(x,y)}}\big) \\
    & = x^N+(y-x^2)h_1(x,y,z)+(z-x^3)h_2(x,y,z).
    \end{align*}
    Thus if $x^{\alpha}y^{\beta}z^{\gamma}\in\II(X)$ then $y-x^2=0=z-x^3$ and the above
    expression reduces to $x^{\alpha}y^{\beta}z^{\gamma}=x^N$. Therefore
    \[
      0=x^{\alpha}y^{\beta}z^{\gamma}|_X=x^N|_X \quad\then\quad
      x^N|_X(t,t^2,t^3)=t^N=0\quad\forall t\in k
    \]
    \[
      \therefore\quad x^{\alpha}y^{\beta}z^{\gamma}=(y-x^2)h_1(x,y,z)+(z-x^3)h_2(x,y,z)\in\gen{y-x^2,z-x^3}.
    \]
    Since this happens for every monomial of $\II(X)$ then it happens for any polynomial
    because $f=\sum_i \la_i x^{\alpha_i}y^{\beta_i}z^{\gamma_i}$. Therefore
    $\II(X)\subseteq\gen{y-x^2,z-x^3}$.
  \item The morphism $\varphi:\AAA^1\ra X$ defined as $\varphi(t)=(t,t^2,t^3)$ is an
    isomorphism with inverse $(t,t^2,t^3)\mapsto t$. Thus $A(X)\cong A(\AAA^1)=k[x]$.
  \end{enumerate}

\begin{figure}[ht] %%%%%%%%%%%%%%%%%%%%%%%%%%%%%%%%%%%%%%%%%%%%%%%%%%%%%%% FIGURA NSIMPLEJOS_GEOMETRICOS
  \centering
  \caption{Twisted Cubic Curve over $k=\RR$}
%  \label{fig:twisted_cubic_curve}
  \begin{subfigure}{0.48\textwidth}
%    \includegraphics[scale=0.4]{twisted_cubic_curve_1}    
  \end{subfigure}
  \begin{subfigure}{0.48\textwidth}
%    \includegraphics[scale=0.35]{twisted_cubic_curve_2}    
  \end{subfigure}
\end{figure}%%%%%%%%%%%%%%%%%%%%%%%%%%%%%%%%%%%%%%%%%%%%%%%%%%%%%%%%%%%%%%%%%%%%%%%%%%%%%%%%%%%%%%%%%%
%
\end{proof}%

